theories/AlgorithmicTyping.v
@@ -3,102 +3,11 @@ From Coq Require Import ssrbool.
 From LogRel.AutoSubst Require Import core unscoped Ast Extra.
 From LogRel Require Import Utils BasicAst Notations Context NormalForms Weakening UntypedReduction GenericTyping DeclarativeTyping.
 
-#[global]
-Instance ren_map_data {Γ Δ} : Ren1 (Δ ≤ Γ) Map.data Map.data :=
-  fun ρ r => Map.mk (Map.srcTy r)⟨ρ⟩ (Map.tgtTy r)⟨ρ⟩ (Map.fn r)⟨ρ⟩ (Map.lst r)⟨ρ⟩.
-
-#[global]
-Instance ren_map_opt {Γ Δ} : Ren1 (Δ ≤ Γ) Map.opt Map.opt :=
-  fun ρ o => match o with | Map.IsMap r => Map.IsMap r⟨ρ⟩ | Map.IsNotMap r => Map.IsNotMap r⟨ρ⟩ end.
-
 Section Definitions.
 
   (** We locally disable typing notations to be able to use them in the definition
   here before declaring the right instance. *)
   Close Scope typing_scope.
-
-
-  Lemma wk_is_map t {Γ Δ} (ρ : Δ ≤ Γ) : is_map t⟨ρ⟩ = is_map t.
-  Proof. now destruct t. Qed.
-
-  Lemma wk_compact_map t: 
-    forall A {Γ Δ} (ρ : Δ ≤ Γ) 
-    (r := compact_map A t) 
-    (r' := compact_map A⟨ρ⟩ t⟨ρ⟩),
-    (Map.srcTy r)⟨ρ⟩ = Map.srcTy r' ×
-    (Map.tgtTy r)⟨ρ⟩ = Map.tgtTy r' ×
-    (Map.fn r)⟨ρ⟩ = Map.fn r' ×
-    (Map.lst r)⟨ρ⟩ = Map.lst r'.
-  Proof.
-    induction t; intros; repeat split; try reflexivity.
-    1,3: eapply IHt4.
-    subst r r'; cbn; f_equal.  1: eapply IHt4.
-    f_equal. 1: now bsimpl.
-    assert (forall x, x⟨↑⟩⟨upRen_term_term ρ⟩ = x⟨ρ⟩⟨↑⟩) as -> by (intros; now bsimpl).
-    do 2 f_equal. eapply IHt4.
-  Qed.
-
-  Lemma compact_map_whne A l :
-    whne (Map.lst (compact_map A l)) -> whne l.
-  Proof.
-    induction l in A |- *; cbn; try easy.
-    intros; constructor; eauto.
-  Qed.
-
-  Lemma wk_map_compact t : forall {Γ Δ} (ρ : Δ ≤ Γ), (Map.compact t)⟨ρ⟩ = Map.compact t⟨ρ⟩.
-  Proof.
-    induction t; intros; try reflexivity; cbn.
-    refold; rewrite <- IHt4.
-    destruct (Map.compact t4); cbn; refold.
-    2: reflexivity.
-    do 2 f_equal. now bsimpl.
-  Qed.
-
-  Lemma wk_map_combine t u : forall {Γ Δ} (ρ : Δ ≤ Γ), 
-    let r := Map.combine t u in let wkr := Map.combine t⟨ρ⟩ u⟨ρ⟩ in 
-    (fst r)⟨ρ⟩ = fst wkr /\ (snd r)⟨ρ⟩ = snd wkr.
-  Proof.
-    unfold Map.combine; intros; destruct t, u; split; reflexivity.
-  Qed.
-
-  Lemma wk_map_extract t u : forall {Γ Δ} (ρ : Δ ≤ Γ), 
-    let r := Map.extract t u in let wkr := Map.extract t⟨ρ⟩ u⟨ρ⟩ in 
-    (fst r)⟨ρ⟩ = fst wkr /\ (snd r)⟨ρ⟩ = snd wkr.
-  Proof.
-    unfold Map.extract; intros.
-    rewrite <- !wk_map_compact.
-    apply wk_map_combine.
-  Qed.
-
-
-  Lemma compact_is_map_whne l r :
-    Map.compact l = Map.IsMap r -> 
-    whne (Map.lst r) -> whne l.
-  Proof.
-    induction l in r |- *; cbn; try (easy + discriminate).
-    destruct (Map.compact l4) eqn:Eq.
-    all:intros [= <-] ?; cbn in *; constructor; tea.
-    eapply IHl4; tea; reflexivity.
-  Qed.
-
-  Lemma compact_is_not_map_whne l r :
-    Map.compact l = Map.IsNotMap r -> 
-    whne r -> whne l.
-  Proof.
-    destruct l; try (cbn; intros [= <-]; easy).
-  Qed.
-
-  Lemma map_extract_whne l l' : 
-    let r := Map.extract l l' in
-    (whne (Map.lst (fst r)) -> whne l) ×
-    (whne (Map.lst (snd r)) -> whne l').
-  Proof.
-    unfold Map.extract.
-    destruct (Map.compact l) eqn:E, (Map.compact l') eqn:E'; cbn.
-    all: try (split; now (apply compact_is_map_whne + apply compact_is_not_map_whne)).
-    split; intros h; inversion h.
-  Qed.
-
 
 (** ** Conversion *)
 
@@ -160,15 +69,6 @@ Section Definitions.
     | neuSndCongAlg {Γ m n A B} :
       [ Γ |- m ~h n ▹ tSig A B ] ->
       [ Γ |- tSnd m ~ tSnd n ▹ B[(tFst m)..] ]
-    | neuMapCompact {Γ A l l'} :
-      let rx := Map.extract l l' in
-      let r := fst rx in
-      let r' := snd rx in
-      is_map l || is_map l' ->
-      [Γ |- r.(Map.lst) ~h r'.(Map.lst) ▹ tList A ] ->
-      [Γ |- r.(Map.tgtTy) ≅ r'.(Map.tgtTy)] ->
-      [Γ |- r.(Map.fn) ≅ r'.(Map.fn) : arr r.(Map.srcTy) r.(Map.tgtTy)] ->
-      [Γ |- l ~ l' ▹ tList r.(Map.tgtTy)]
   (** **** Conversion of neutral terms at a type reduced to weak-head normal form*)
   with ConvNeuRedAlg : context -> term -> term -> term -> Type :=
     | neuConvRed {Γ m n A A'} :
@@ -177,22 +77,21 @@ Section Definitions.
       whnf A' ->
       [Γ |- m ~h n ▹ A']
 
-  (** **** Conversion of neutral terms at a positive type *)
-  (* [Γ |- m ~ n ◃ P ] 
+  (** **** Conversion of neutral lists *)
+  (* [Γ |- m ~ n :List A ] 
     Presupposes:
-      [|-[de] Γ], [Γ |-[de] P], [Γ |-[de] m : P], [Γ |-[de] n : P]
+      [|-[de] Γ], [Γ |-[de] A], [Γ |-[de] m : tList A], [Γ |-[de] n : tList A]
     Ensures: 
-      positive P
+      [Γ |- m ≅ n : tList A]
   *)
-  (* with ConvNeuPosAlg : context -> term -> term -> term -> Type :=
-    | neuNat {Γ A n n'} : [Γ |- n ~ n' ▹ A] -> [Γ |- n ~ n' ◃ tNat]
-    | neuMapCompact {Γ A B l l'} :
-      (* compact_map reduces all maps in head position, possibly inserting an identity *)
-      let r := compact_map B l in
-      let r' := compact_map B l' in
-      [Γ |- r.(Map.lst) ~h r'.(Map.lst) ▹ tList A ] ->
-      [Γ |- r.(Map.fn) ≅ r'.(Map.fn) : arr A B] ->
-      [Γ |- l ~ l' ◃ tList B] *)
+  with ConvNeuListAlg : context -> term -> term -> term -> Type :=
+  | neuMapCompact {Γ A B l l'} :
+    (* Map.compact reduces all maps in head position, possibly inserting an identity *)
+    let r := Map.compact B l in
+    let r' := Map.compact B l' in
+    [Γ |- r.(Map.lst) ~h r'.(Map.lst) ▹ tList A ] ->
+    [Γ |- r.(Map.fn) ≅ r'.(Map.fn) : arr A B] ->
+    [Γ |- l ~ l' :List B]
 
   (** **** Conversion of terms *)
   with ConvTermAlg : context -> term -> term -> term -> Type :=
@@ -242,13 +141,13 @@ Section Definitions.
       [Γ |- hd ≅ hd' : A] ->
       [Γ |- tl ≅ tl' : tList A] ->
       [Γ |- tCons A hd tl ≅h tCons A' hd' tl' : tList AT]
+    | termListNeuConvAlg {Γ m n A} :
+      [Γ |- m ~ n :List A] ->
+      [Γ |- m ≅h n : tList A]
     | termNeuConvAlg {Γ m n T P} :
       [Γ |- m ~ n ▹ T] ->
       isPosType P ->
       [Γ |- m ≅h n : P]
-    (* | termNeuConvAlg {Γ m n P} :
-      [Γ |- m ~ n ◃ P] ->
-      [Γ |- m ≅h n : P] *)
 
   where "[ Γ |- A ≅ B ]" := (ConvTypeAlg Γ A B)
   and "[ Γ |- A ≅h B ]" := (ConvTypeRedAlg Γ A B)
@@ -256,7 +155,7 @@ Section Definitions.
   and "[ Γ |- m ~h n ▹ T ]" := (ConvNeuRedAlg Γ T m n)
   and "[ Γ |- t ≅ u : T ]" := (ConvTermAlg Γ T t u)
   and "[ Γ |- t ≅h u : T ]" := (ConvTermRedAlg Γ T t u)
-  (* and "[ Γ |- m ~ n ◃ T]" := (ConvNeuPosAlg Γ T m n) *)
+  and "[ Γ |- m ~ n :List A ]" := (ConvNeuListAlg Γ A m n)
   and "[ t ⇒ t' ]" := (OneRedAlg t t')
   and "[ t ⇒* t' ]" := (RedClosureAlg t t').
 
@@ -396,6 +295,7 @@ Module AlgorithmicTypingData.
   #[export] Instance ConvTermRed_Algo : ConvTermRed al := ConvTermRedAlg.
   #[export] Instance ConvNeu_Algo : ConvNeu al := ConvNeuAlg.
   #[export] Instance ConvNeuRed_Algo : ConvNeuRed al := ConvNeuRedAlg.
+  #[export] Instance ConvNeuList_Algo : ConvNeuList al := ConvNeuListAlg.
 
   Ltac fold_algo :=
     change WfContextAlg with (wf_context (ta := al)) in * ;
@@ -410,7 +310,8 @@ Module AlgorithmicTypingData.
     change ConvNeuAlg with (conv_neu (ta := al)) in * ;
     change ConvTypeRedAlg with (conv_type_red (ta := al)) in * ;
     change ConvTermRedAlg with (conv_term_red (ta := al)) in * ;
-    change ConvNeuRedAlg with (conv_neu_red (ta := al)) in *.
+    change ConvNeuRedAlg with (conv_neu_red (ta := al)) in * ;
+    change ConvNeuListAlg with (conv_neu_list (ta := al)) in *.
 
   Smpl Add fold_algo : refold.
 
@@ -429,6 +330,7 @@ Scheme
     Minimality for ConvTypeRedAlg Sort Type with
     Minimality for ConvNeuAlg Sort Type with
     Minimality for ConvNeuRedAlg Sort Type with
+    Minimality for ConvNeuListAlg Sort Type with
     Minimality for ConvTermAlg Sort Type with
     Minimality for ConvTermRedAlg Sort Type.
 
@@ -443,6 +345,7 @@ Combined Scheme _AlgoConvInduction from
     ConvTypeRedAlg_rect_nodep,
     ConvNeuAlg_rect_nodep,
     ConvNeuRedAlg_rect_nodep,
+    ConvNeuListAlg_rect_nodep,
     ConvTermAlg_rect_nodep,
     ConvTermRedAlg_rect_nodep.
 
@@ -467,8 +370,8 @@ Let AlgoConvInductionType :=
 
 Lemma AlgoConvDefInduction : AlgoConvInductionType.
 Proof.
-  intros PTyEq PTyRedEq PNeEq PNeRedEq PTmEq PTmRedEq **.
-  pose proof (_AlgoConvInduction PTyEq PTyRedEq PNeEq PNeRedEq PTmEq PTmRedEq) as H.
+  intros PTyEq PTyRedEq PNeEq PNeRedEq PNeListEq PTmEq PTmRedEq **.
+  pose proof (_AlgoConvInduction PTyEq PTyRedEq PNeEq PNeRedEq PNeListEq PTmEq PTmRedEq) as H.
   destruct H as [?[?[?[?[?]]]]] ; cycle -1.
   1: by_prod_splitter.
   all: assumption.
@@ -476,8 +379,8 @@ Defined.
 
 Lemma AlgoConvInduction : AlgoConvInductionType.
 Proof.
-  intros PTyEq PTyRedEq PNeEq PNeRedEq PTmEq PTmRedEq **.
-  pose proof (_AlgoConvInduction PTyEq PTyRedEq PNeEq PNeRedEq PTmEq PTmRedEq) as H.
+  intros PTyEq PTyRedEq PNeEq PNeRedEq PNeListEq PTmEq PTmRedEq **.
+  pose proof (_AlgoConvInduction PTyEq PTyRedEq PNeEq PNeRedEq PNeListEq PTmEq PTmRedEq) as H.
   destruct H as [?[?[?[?[?]]]]] ; cycle -1.
   1: by_prod_splitter.
   all: assumption.
@@ -524,340 +427,10 @@ Definition AlgoTypingInductionConcl :=
     let t' := remove_steps t in
     exact t').
 
-Scheme 
-    ConvTypeAlg_rect_dep := Induction for ConvTypeAlg Sort Type with
-    ConvTypeRedAlg_rect_dep := Induction for ConvTypeRedAlg Sort Type with
-    ConvNeuAlg_rect_dep := Induction for ConvNeuAlg Sort Type with
-    ConvNeuRedAlg_rect_dep := Induction for ConvNeuRedAlg Sort Type with
-    ConvTermAlg_rect_dep := Induction for ConvTermAlg Sort Type with
-    ConvTermRedAlg_rect_dep := Induction for ConvTermRedAlg Sort Type.
-
-Scheme
-    WfTypeAlg_rect_dep := Induction for WfTypeAlg Sort Type with
-    InferAlg_rect_dep := Induction for InferAlg Sort Type with
-    InferRedAlg_rect_dep := Induction for InferRedAlg Sort Type with
-    CheckAlg_rect_dep := Induction for CheckAlg Sort Type.
-
-Combined Scheme _AlgoConvDepInduction from
-    ConvTypeAlg_rect_dep,
-    ConvTypeRedAlg_rect_dep,
-    ConvNeuAlg_rect_dep,
-    ConvNeuRedAlg_rect_dep,
-    ConvTermAlg_rect_dep,
-    ConvTermRedAlg_rect_dep.
-
-Combined Scheme _AlgoTypingDepInduction from
-    WfTypeAlg_rect_dep,
-    InferAlg_rect_dep,
-    InferRedAlg_rect_dep,
-    CheckAlg_rect_dep.
-
-Let _AlgoConvDepInductionType :=
-  ltac:(let ind := fresh "ind" in
-      pose (ind := _AlgoConvDepInduction);
-      refold ;
-      let ind_ty := type of ind in
-      exact ind_ty).
-
-Let AlgoConvDepInductionType :=
-  ltac: (let ind := eval cbv delta [_AlgoConvDepInductionType] zeta
-    in _AlgoConvDepInductionType in
-    let ind' := polymorphise ind in
-  exact ind').
-
-Lemma AlgoConvDepInduction : AlgoConvDepInductionType.
-Proof.
-  intros PTyEq PTyRedEq PNeEq PNeRedEq PTmEq PTmRedEq **.
-  pose proof (_AlgoConvDepInduction PTyEq PTyRedEq PNeEq PNeRedEq PTmEq PTmRedEq) as H.
-  destruct H as [?[?[?[?[?]]]]] ; cycle -1.
-  1: by_prod_splitter.
-  all: assumption.
-Qed.
-
-Let _AlgoTypingDepInductionType :=
-  ltac:(let ind := fresh "ind" in
-      pose (ind := _AlgoTypingDepInduction);
-      refold ;
-      let ind_ty := type of ind in
-      exact ind_ty).
-
-Let AlgoTypingDepInductionType :=
-  ltac: (let ind := eval cbv delta [_AlgoTypingDepInductionType] zeta
-    in _AlgoTypingDepInductionType in
-    let ind' := polymorphise ind in
-  exact ind').
-
-Lemma AlgoTypingDepInduction : AlgoTypingDepInductionType.
-Proof.
-  intros PTy PInf PInfRed PCheck **.
-  pose proof (_AlgoTypingDepInduction PTy PInf PInfRed PCheck) as H.
-  destruct H as [?[?[?]]] ; cycle -1.
-  1: by_prod_splitter.
-  all: assumption.
-Qed.
-
-Definition AlgoConvDepInductionConcl :=
-  ltac:(
-    let t := eval cbv delta [AlgoConvDepInductionType] beta in AlgoConvDepInductionType in
-    let t' := remove_steps t in
-    exact t').
-
-Definition AlgoTypingDepInductionConcl :=
-  ltac:(
-    let t := eval cbv delta [AlgoTypingDepInductionType] beta in AlgoTypingDepInductionType in
-    let t' := remove_steps t in
-    exact t').
-
 End InductionPrinciples.
 
 Arguments AlgoConvInductionConcl PTyEq PTyRedEq PNeEq PNeRedEq PTmEq PTmRedEq : rename.
 Arguments AlgoTypingInductionConcl PTy PInf PInfRed PCheck : rename.
-Arguments AlgoConvDepInductionConcl PTyEq PTyRedEq PNeEq PNeRedEq PTmEq PTmRedEq : rename.
-Arguments AlgoTypingDepInductionConcl PTy PInf PInfRed PCheck : rename.
-
-(** ** Size of a derivation for well-founded inductions *)
-
-Class Sized A := size : A -> nat.
-Notation "#| x |" := (size x).
-
-Section Size.
-  Import AlgorithmicTypingData.
-  
-  Let PTyEq (Γ : context) (A B : term) := nat.
-  Let PTyRedEq (Γ : context) (A B : term) := nat.
-  Let PNeEq (Γ : context) (A t u : term) := nat.
-  Let PNeRedEq (Γ : context) (A t u : term) := nat.
-  Let PTmEq (Γ : context) (A t u : term) := nat.
-  Let PTmRedEq (Γ : context) (A t u : term) := nat.
-
-  #[local]
-  Ltac sum :=
-    match goal with
-    | |- nat => refine (S _)
-    | |- nat -> _ => let n := fresh "n" in intro n; sum; refine (n + _)
-    end.
-
-  Theorem algo_conv_size :
-    _AlgoConvInductionConcl PTyEq PTyRedEq
-      PNeEq PNeRedEq PTmEq PTmRedEq.
-  Proof.
-    subst PTyEq PTyRedEq PNeEq PNeRedEq PTmEq PTmRedEq.
-    apply _AlgoConvInduction; intros;
-      repeat match goal with
-      | [H : nat |- _] => revert H
-      | [H : _ |- _] => clear H
-      end; sum; exact 0.
-  Defined.
-    
-End Size.
-
-#[global] Instance ConvTypeAlgSized Γ A B : Sized (ConvTypeAlg Γ A B). Proof. unfold Sized; apply algo_conv_size. Defined.
-#[global] Instance ConvTypeRedAlgSized Γ A B : Sized (ConvTypeRedAlg Γ A B). Proof. unfold Sized; apply algo_conv_size. Defined.
-#[global] Instance ConvNeuAlgSized Γ A t u : Sized (ConvNeuAlg Γ A t u). Proof. unfold Sized; apply algo_conv_size. Defined.
-#[global] Instance ConvNeuRedAlgSized Γ A t u : Sized (ConvNeuRedAlg Γ A t u). Proof. unfold Sized; apply algo_conv_size. Defined.
-#[global] Instance ConvTermAlgSized Γ A t u : Sized (ConvTermAlg Γ A t u). Proof. unfold Sized; apply algo_conv_size. Defined.
-#[global] Instance ConvTermRedAlgSized Γ A t u: Sized (ConvTermRedAlg Γ A t u). Proof. unfold Sized; apply algo_conv_size. Defined.
-
-Section SizeLemmas.
-  Import AlgorithmicTypingData.
-  
-  Lemma typeConvRed_size Γ A A' B B'
-    (redA : [A ⇒* A'])
-    (redB : [B ⇒* B'])
-    (conv : [Γ |- A' ≅h B']) :
-    #|typeConvRed redA redB conv| = S (#|conv| + 0).
-  Proof. reflexivity. Qed.
-
-  
-  Lemma typePiCongAlg_size  Γ A B A' B'
-    (convA : [ Γ |- A ≅ A'])
-    (convB : [ Γ ,, A |- B ≅ B']) :
-    #|typePiCongAlg convA convB| = S (#|convB| + (#|convA| + 0)).
-  Proof. reflexivity. Qed. 
-  
-  Lemma typeUnivConvAlg_size  Γ :
-    #|@typeUnivConvAlg Γ| = 1.
-  Proof. reflexivity. Qed.
-
-  Lemma typeNatConvAlg_size  Γ :
-    #|@typeNatConvAlg Γ| = 1.
-  Proof. reflexivity. Qed.
-
-  Lemma typeEmptyConvAlg_size  Γ :
-    #|@typeEmptyConvAlg Γ| = 1.
-  Proof. reflexivity. Qed.
-
-  Lemma typeSigCongAlg_size  Γ A B A' B'
-    (convA : [ Γ |- A ≅ A'])
-    (convB : [ Γ ,, A |- B ≅ B']) :
-    #|typeSigCongAlg convA convB| = S(#|convB| + (#|convA| + 0)).
-  Proof. reflexivity. Qed.
-
-  Lemma typeListCongAlg_size  Γ A A'
-    (convA :[Γ |- A ≅ A']) :
-    #|typeListCongAlg convA| = S (#|convA| + 0).
-  Proof. reflexivity. Qed.
-
-  Lemma typeNeuConvAlg_size  Γ M N T
-    (inf : [ Γ |- M ~ N ▹ T]) :
-    #|typeNeuConvAlg inf| = S (#|inf| + 0).
-  Proof. reflexivity. Qed.
-
-Lemma neuVarConvAlg_size  Γ n decl
-    (hn : in_ctx Γ n decl) :
-    #|neuVarConvAlg hn| = S (n + 0).
-Proof. reflexivity. Qed.
-
-Lemma neuAppCongAlg_size  Γ m n t u A B
-    (convFun : [ Γ |- m ~h n ▹ tProd A B ])
-    (convArg : [ Γ |- t ≅ u : A ]) :
-    #|neuAppCongAlg convFun convArg| = S (#|convArg| + (#|convFun| + 0)).
-Proof. reflexivity. Qed.
-
-Lemma neuNatElimCong_size  Γ n n' P P' hz hz' hs hs'
-  (convn : [Γ |- n ~h n' ▹ tNat])
-  (convP : [Γ,, tNat |- P ≅ P'])
-  (convhz : [Γ |- hz ≅ hz' : P[tZero..]])
-  (convhs : [Γ |- hs ≅ hs' : elimSuccHypTy P]) :
-  #|neuNatElimCong convn convP convhz convhs| = S(#|convhs| + (#|convhz| + (#|convP| + (#|convn| + 0)))).
-  Proof. reflexivity. Qed.
-
-Lemma neuEmptyElimCong_size  Γ P P' e e'
-    (conve : [Γ |- e ~h e' ▹ tEmpty])
-    (convP : [Γ ,, tEmpty |- P ≅ P']) :
-    #|neuEmptyElimCong conve convP| = S(#|convP| + (#|conve| + 0)).
-  Proof. reflexivity. Qed.
-
-Lemma neuFstCongAlg_size  Γ m n A B 
-    (convm : [ Γ |- m ~h n ▹ tSig A B ]) :
-    #|neuFstCongAlg convm| = S(#|convm| + 0).
-  Proof. reflexivity. Qed.
-
-Lemma neuSndCongAlg_size  Γ m n A B 
-    (convm : [ Γ |- m ~h n ▹ tSig A B ]) :
-    #|neuSndCongAlg convm| = S(#|convm| + 0).
-  Proof. reflexivity. Qed.
-
-Lemma neuMapCompact_size  Γ A l l'
-    (rx := Map.extract l l') (r := fst rx) (r' := snd rx)
-    (hmap : is_map l || is_map l')
-    (convlst : [Γ |- r.(Map.lst) ~h r'.(Map.lst) ▹ tList A ])
-    (convtgtty : [Γ |- r.(Map.tgtTy) ≅ r'.(Map.tgtTy)])
-    (convfn : [Γ |- r.(Map.fn) ≅ r'.(Map.fn) : arr r.(Map.srcTy) r.(Map.tgtTy)]) :
-    #|neuMapCompact hmap convlst convtgtty convfn| = S(#|convfn| + (#|convtgtty| + (#|convlst| + 0))).
-  Proof. reflexivity. Qed.
-
-Lemma neuConvRed_size  Γ m n A A'
-    (conv : [Γ |- m ~ n ▹ A])
-    (redA : [A ⇒* A'])
-    (whA : whnf A') :
-  #|neuConvRed conv redA whA| = S(#|conv| + 0).
-  Proof. reflexivity. Qed.
-
-Lemma termConvRed_size  Γ t t' u u' A A'
-      (redA : [A ⇒* A'])
-      (redt : [t ⇒* t'])
-      (redu : [u ⇒* u' ])
-      (conv : [Γ |- t' ≅h u' : A']) :
-      #|termConvRed redA redt redu conv| = S(#|conv| + 0).
-    Proof. reflexivity. Qed.
-Lemma termPiCongAlg_size  Γ A B A' B'
-      (convA : [ Γ |- A ≅ A' : U])
-      (convB : [ Γ ,, A |- B ≅ B' : U]) :
-      #|termPiCongAlg convA convB| = S(#|convB| + (#|convA| + 0)).
-    Proof. reflexivity. Qed.
-Lemma termNatReflAlg_size  Γ :
-  #|@termNatReflAlg Γ| = 1.
-    Proof. reflexivity. Qed.
-Lemma termZeroReflAlg_size  Γ :
-      #|@termZeroReflAlg Γ| = 1.
-    Proof. reflexivity. Qed.
-Lemma termSuccCongAlg_size  Γ t t'
-    (convt : [Γ |- t ≅ t' : tNat]) :
-    #|termSuccCongAlg convt| = S(#|convt| + 0).
-    Proof. reflexivity. Qed.
-Lemma termEmptyReflAlg_size  Γ :
-#|@termEmptyReflAlg Γ| = 1.
-    Proof. reflexivity. Qed.
-Lemma termFunConvAlg_size  Γ f g A B
-      (whf :whnf f)
-      (whg : whnf g)
-      (conveta : [ Γ,, A |- eta_expand f ≅ eta_expand g : B]) :
-      #|termFunConvAlg whf whg conveta| = S(#|conveta| + 0).
-    Proof. reflexivity. Qed.
-Lemma termSigCongAlg_size  Γ A B A' B'
-    (convA : [ Γ |- A ≅ A' : U])
-    (convB : [ Γ ,, A |- B ≅ B' : U]) :
-    #|termSigCongAlg convA convB| = S(#|convB| + (#|convA| + 0)).
-    Proof. reflexivity. Qed.
-Lemma termPairConvAlg_size  Γ p q A B
-      (whp : whnf p)
-      (whq : whnf q)
-      (convfst : [ Γ |- tFst p ≅ tFst q : A])
-      (convsnd : [ Γ |- tSnd p ≅ tSnd q : B[(tFst p)..]]) :
-      #|termPairConvAlg whp whq convfst convsnd| = S(#|convsnd| + (#|convfst| + 0)).
-    Proof. reflexivity. Qed.
-Lemma termListCongAlg_size  Γ A A'
-      (convA : [Γ |- A ≅ A' : U]) :
-      #|termListCongAlg convA| = S(#|convA| + 0).
-    Proof. reflexivity. Qed.
-Lemma termNilConvAlg_size  Γ A A' AT :
-      #|@termNilConvAlg Γ A A' AT| = 1.
-    Proof. reflexivity. Qed.
-Lemma termConsCongAlg_size  Γ A A' AT hd hd' tl tl'
-      (convhd : [Γ |- hd ≅ hd' : A])
-      (convtl : [Γ |- tl ≅ tl' : tList A]) :
-      #|termConsCongAlg A' AT convhd convtl| = S(#|convtl| + (#|convhd| + 0)).
-    Proof. reflexivity. Qed.
-Lemma termNeuConvAlg_size  Γ m n T P
-      (inf : [Γ |- m ~ n ▹ T])
-      (ispos : isPosType P) :
-      #|termNeuConvAlg inf ispos| = S(#|inf| + 0).
-    Proof. reflexivity. Qed.
-
-End SizeLemmas.
-
-Create HintDb sizeLemmas.
-#[global]
-Hint Rewrite typeConvRed_size typePiCongAlg_size typeUnivConvAlg_size typeNatConvAlg_size typeEmptyConvAlg_size typeSigCongAlg_size typeListCongAlg_size typeNeuConvAlg_size neuVarConvAlg_size neuAppCongAlg_size neuNatElimCong_size neuEmptyElimCong_size neuFstCongAlg_size neuSndCongAlg_size neuMapCompact_size neuConvRed_size termConvRed_size termPiCongAlg_size termNatReflAlg_size termZeroReflAlg_size termSuccCongAlg_size termEmptyReflAlg_size termFunConvAlg_size termSigCongAlg_size termPairConvAlg_size termListCongAlg_size termNilConvAlg_size termConsCongAlg_size termNeuConvAlg_size : sizeLemmas.
-
-Ltac simpl_size := autorewrite with sizeLemmas; refold.
-
-Arguments algo_conv_size : simpl never.
-Arguments size : simpl never.
-
-From Coq Require Import Lia.
-
-Section SizeAtLeastOne.
-  Import AlgorithmicTypingData.
-
-  Let PTy Γ A B (h : [Γ |-[al] A ≅ B]) := 1 <= #|h|.
-  Let PTyRed Γ A B (h : [Γ |-[al] A ≅h B]) := 1 <= #|h|.
-  Let PNe Γ A m n (h : [Γ |-[al] m ~ n ▹ A]) := 1 <= #|h|.
-  Let PNeRed Γ A m n (h : [Γ |-[al] m ~h n ▹ A]) := 1 <= #|h|.
-  Let PTm Γ A t u (h : [Γ |-[al] t ≅ u : A]) := 1 <= #|h|.
-  Let PTmRed Γ A t u (h : [Γ |-[al] t ≅h u : A]) := 1 <= #|h|.
-
-  Lemma size_positive : AlgoConvDepInductionConcl PTy PTyRed PNe PNeRed PTm PTmRed.
-  Proof.
-    subst PTy PTyRed PNe PNeRed PTm PTmRed.
-    eapply AlgoConvDepInduction; intros; simpl_size; lia.
-  Qed.
-End SizeAtLeastOne.
-(* Section Foo.
-  Import AlgorithmicTypingData.
-  From Coq Require Import Lia.
-  Goal forall Γ A B (h : [Γ |-[al] A ≅ B]), True.
-  Proof.
-      intros.
-      pose (h' := h).
-      destruct h.
-      assert (#|c| < #| h'|).
-      unfold h'; cbn.
-      unfold h'; simpl_size. lia.
-
-
-End Foo. *)
 
 
 (** ** Stability by weakening *)
@@ -873,6 +446,8 @@ Section TypingWk.
     [Δ |- t⟨ρ⟩ ~ u⟨ρ⟩ ▹ A⟨ρ⟩].
   Let PNeRedEq (Γ : context) (A t u : term) := forall Δ (ρ : Δ ≤ Γ),
     [Δ |- t⟨ρ⟩ ~h u⟨ρ⟩ ▹ A⟨ρ⟩].
+    Let PNeListEq (Γ : context) (A t u : term) := forall Δ (ρ : Δ ≤ Γ),
+      [Δ |- t⟨ρ⟩ ~ u⟨ρ⟩ :List A⟨ρ⟩].
   Let PTmEq (Γ : context) (A t u : term) := forall Δ (ρ : Δ ≤ Γ),
     [Δ |- t⟨ρ⟩ ≅ u⟨ρ⟩ : A⟨ρ⟩].
   Let PTmRedEq (Γ : context) (A t u : term) := forall Δ (ρ : Δ ≤ Γ),
@@ -880,9 +455,9 @@ Section TypingWk.
 
   Theorem algo_conv_wk :
     AlgoConvInductionConcl PTyEq PTyRedEq
-      PNeEq PNeRedEq PTmEq PTmRedEq.
+      PNeEq PNeRedEq PNeListEq PTmEq PTmRedEq.
   Proof.
-    subst PTyEq PTyRedEq PNeEq PNeRedEq PTmEq PTmRedEq.
+    subst PTyEq PTyRedEq PNeEq PNeRedEq PNeListEq PTmEq PTmRedEq.
     apply AlgoConvInduction.
     - intros.
       econstructor.
@@ -944,28 +519,19 @@ Section TypingWk.
     - intros ??? A? ? IH *; cbn.
       rewrite (subst_ren_wk_up (A:=A)).
       econstructor; now eapply IH.
-    - intros *.
-      intros ? ? ihlst ? ihtgt ? ihfn *.
-      pose proof (wk_map_extract l l' ρ) as [fsteq sndeq].
-      rewrite <- wk_list.
-      change (Map.tgtTy ?x)⟨ρ⟩ with (Map.tgtTy x⟨ρ⟩).
-      rewrite fsteq.
-      eapply neuMapCompact; refold; rewrite <- ?fsteq, <- ?sndeq.
-      + now do 2 rewrite wk_is_map.
-      + eapply convne_meta_conv.
-        1: eapply ihlst.
-        1: reflexivity.
-        now symmetry.
-      + eapply ihtgt.
-      + eapply convtm_meta_conv.
-        1: eapply ihfn.
-        2: now symmetry.
-        now bsimpl.
     - intros.
       econstructor.
       + eauto.
       + eauto using credalg_wk.
-      + gen_typing. 
+      + gen_typing.
+    - intros * ? ihlst ? ihfn *.
+      cbn.
+      econstructor.
+      all: repeat rewrite <- wk_map_compact.
+      + cbn in ihlst.
+        apply ihlst.
+      + refold. rewrite wk_arr.
+        now apply ihfn.
     - intros.
       econstructor.
       1-3: eauto using credalg_wk.
@@ -1006,9 +572,11 @@ Section TypingWk.
     - intros; cbn.
       econstructor; eauto.
     - intros.
+      now econstructor.
+    - intros.
       econstructor.
       + eauto.
-      + eauto using isPosType_ren.
+      + gen_typing. 
   Qed.
 
   Let PTy (Γ : context) (A : term) := forall Δ (ρ : Δ ≤ Γ), [Δ |- A⟨ρ⟩].
@@ -1125,6 +693,7 @@ Section TypingWk.
       (fun (Γ : context) (A B : term) => forall T, [Γ,, T |- A⟨↑⟩ ≅h B⟨↑⟩])
       (fun (Γ : context) (A m n : term) => forall T, [Γ,, T |- m⟨↑⟩ ~ n⟨↑⟩ ▹ A⟨↑⟩])
       (fun (Γ : context) (A m n : term) => forall T, [Γ,, T |- m⟨↑⟩ ~h n⟨↑⟩ ▹ A⟨↑⟩])
+      (fun (Γ : context) (A m n : term) => forall T, [Γ,, T |- m⟨↑⟩ ~ n⟨↑⟩ :List A⟨↑⟩])
       (fun (Γ : context) (A t u : term) => forall T, [Γ,, T |- t⟨↑⟩ ≅ u⟨↑⟩ : A⟨↑⟩])
       (fun (Γ : context) (A t u : term) => forall T, [Γ,, T |- t⟨↑⟩ ≅h u⟨↑⟩ : A⟨↑⟩]).
   Proof.
@@ -1167,18 +736,21 @@ Section AlgTypingWh.
     whne t × whne u.
   Let PNeRedEq (Γ : context) (A t u : term) :=
     [× whne t, whne u & whnf A].
+  Let PNeListEq (Γ : context) (A t u : term) :=
+    whne_list t × whne_list u.
   Let PTmEq (Γ : context) (A t u : term) := True.
   Let PTmRedEq (Γ : context) (A t u : term) := 
     [× whnf t, whnf u & isType A].
 
   Theorem algo_conv_wh :
-    AlgoConvInductionConcl PTyEq PTyRedEq PNeEq PNeRedEq PTmEq PTmRedEq.
+    AlgoConvInductionConcl PTyEq PTyRedEq PNeEq PNeRedEq PNeListEq PTmEq PTmRedEq.
   Proof.
-    subst PTyEq PTyRedEq PNeEq PNeRedEq PTmEq PTmRedEq; cbn.
+    subst PTyEq PTyRedEq PNeEq PNeRedEq PNeListEq PTmEq PTmRedEq; cbn.
     apply AlgoConvInduction.
     all: intros ; prod_splitter ; prod_hyp_splitter.
-    all: try solve [now constructor| now eapply (map_extract_whne l l')].
-    all: gen_typing.
+    all: try solve [now constructor].
+    all: try solve [gen_typing].
+    all: eauto using compact_map_whne with gen_typing.
   Qed.
 End AlgTypingWh.
 
@@ -1195,49 +767,37 @@ Let PNeEq (Γ : context) (A t u : term) :=
   forall A', [Γ |-[al] t ~ u ▹ A'] -> A' = A.
 Let PNeRedEq (Γ : context) (A t u : term) :=
   forall A', [Γ |-[al] t ~h u ▹ A'] -> A' = A.
+Let PNeListEq (Γ : context) (A t u : term) := True.
 Let PTmEq (Γ : context) (A t u : term) := True.
 Let PTmRedEq (Γ : context) (A t u : term) := True.
 
-  Ltac no_map :=
-    match goal with [H : context c [is_map _] |- _] => cbn in H; inversion H end.
-
-
 Theorem algo_conv_det :
-  AlgoConvInductionConcl PTyEq PTyRedEq PNeEq PNeRedEq PTmEq PTmRedEq.
+  AlgoConvInductionConcl PTyEq PTyRedEq PNeEq PNeRedEq PNeListEq PTmEq PTmRedEq.
 Proof.
-  subst PTyEq PTyRedEq PNeEq PNeRedEq PTmEq PTmRedEq; cbn.
+  subst PTyEq PTyRedEq PNeEq PNeRedEq PNeListEq PTmEq PTmRedEq; cbn.
   apply AlgoConvInduction.
   all: try easy.
   - intros * ? * Hconv.
     inversion Hconv ; subst ; clear Hconv.
-    2: no_map.
     now eapply in_ctx_inj.
   - intros * ? IH ? _ ? Hconv.
     inversion Hconv ; subst ; clear Hconv ; refold.
-    2: no_map.
     apply IH in H6.
     now inversion H6.
   - intros * ? IH ????? _ ? Hconv.
     inversion Hconv ; subst ; clear Hconv ; refold.
-    2: no_map.
     now reflexivity.
   - intros * ? IH ?? ? Hconv.
     inversion Hconv ; subst ; clear Hconv ; refold.
-    2: no_map.
     now reflexivity.
   - intros * ? IH ? Hconv.
     inversion Hconv; subst; clear Hconv; refold.
-    2: no_map.
     apply IH in H4.
     now inversion H4.
   - intros * ? IH ? Hconv.
     inversion Hconv; subst; clear Hconv; refold.
-    2: no_map.
     apply IH in H4.
     now inversion H4.
-  - intros * hmap ? ih ? _ ? _ ? Hconv.
-    inversion Hconv; subst; clear Hconv; refold; try no_map.
-    reflexivity.
   - intros * ? IH ??? Hconv.
     inversion Hconv ; subst ; clear Hconv ; refold.
     eapply IH in H2 as ->.
@@ -1306,188 +866,3 @@ Proof.
 Qed.
 
 End AlgoTypingDet.
-
-(*
-From Coq Require Import Lia.
-From Equations Require Import Equations.
-
-Derive Signature for ConvTypeAlg.
-Derive Signature for ConvTypeRedAlg.
-Derive Signature for ConvNeuAlg.
-Derive Signature for ConvNeuRedAlg.
-Derive Signature for ConvTermAlg.
-Derive Signature for ConvTermRedAlg.
-
-Derive NoConfusion for term.
-Derive NoConfusion for sort.
-Derive NoConfusion for nat.
-Derive NoConfusion for list.
-Derive NoConfusion for in_ctx.
-
-#[global]
-Instance: UIP nat. Proof. typeclasses eauto. Defined.
-
-Section SizeUnicity.
-  Import AlgorithmicTypingData.
-
-  (* Definition G := (cons (tList tNat) nil).
-  Definition G' := (cons (tList (tApp (idterm U) tNat)) nil).
-  Definition t := tRel 0.
-  Definition u := tMap tNat tNat (idterm tNat) t.
-
-  Definition f : [G |- t ~ u ▹ tList tNat].
-  Proof.
-    pose (r := compact_map tNat t).
-    pose (r' := compact_map tNat u).
-    change tNat with (Map.tgtTy r).
-    econstructor; cbn; refold.
-    1:easy.
-    - econstructor; refold.
-      2: reflexivity.
-      2: constructor.
-      do 2 econstructor.
-    - econstructor; refold.
-      1,2: reflexivity.
-      econstructor.
-    - econstructor; refold.
-      1-3: reflexivity.
-      econstructor; refold.
-      1,2: constructor.
-      econstructor; refold.
-      1: reflexivity.
-      1: apply redalg_one_step; constructor.
-      + etransitivity.
-        1: apply redalg_one_step; constructor.
-        refold; cbn.
-        etransitivity.
-        1: apply redalg_one_step; constructor.
-        cbn.
-        1: apply redalg_one_step; constructor.
-      + refold. cbn.
-        econstructor; refold.
-        2: constructor.
-        econstructor.
-        constructor.
-  Defined.
-
-  Definition f' : [G' |- t ~ u ▹ tList (tApp (idterm U) tNat)].
-  Proof.
-    pose (r := compact_map (tApp (idterm U) tNat) t).
-    pose (r' := compact_map (tApp (idterm U) tNat) u).
-    change (tApp _ _) with (Map.tgtTy r).
-    econstructor; cbn; refold.
-    1:easy.
-    - econstructor; refold.
-      2: reflexivity.
-      2: constructor.
-      econstructor.
-      do 2 econstructor.
-    - econstructor; refold.
-      1: apply redalg_one_step; constructor.
-      1: reflexivity.
-      cbn; econstructor.
-    - econstructor; refold.
-      1-3: reflexivity.
-      econstructor; refold.
-      1,2: constructor.
-      econstructor; refold.
-      1,2: apply redalg_one_step; constructor.
-      + etransitivity.
-        1: apply redalg_one_step; constructor.
-        refold; cbn.
-        etransitivity.
-        1: apply redalg_one_step; constructor.
-        cbn.
-        1: apply redalg_one_step; constructor.
-      + refold. cbn.
-        econstructor; refold.
-        2: constructor.
-        econstructor.
-        constructor.
-  Defined.
-
-  Lemma foo : #|f| = #|f'|.
-  Proof. reflexivity. Qed. *)
-
-  
-  Let PTyEq (Γ : context) (A B : term) (h1 : [Γ |- A ≅ B]) := 
-    forall Δ (h2 : [Δ |- A ≅ B]), #|h1| = #|h2|.
-  Let PTyRedEq (Γ : context) (A B : term) (h1 : [Γ |- A ≅h B]) := 
-    forall Δ (h2: [Δ |- A ≅h B]), #|h1| = #|h2|.
-  Let PNeEq (Γ : context) (A t u : term) (h1: [Γ |- t ~ u ▹ A]) := 
-    forall Δ B (h2: [Δ |- t ~ u ▹ B]), #|h1| = #|h2|.
-  Let PNeRedEq (Γ : context) (A t u : term) (h1: [Γ |- t ~h u ▹ A]) := 
-    forall Δ B (h2: [Δ |- t ~h u ▹ B]), #|h1| = #|h2|.
-  Let PTmEq (Γ : context) (A t u : term) (h1: [Γ |- t ≅ u : A]) :=
-    forall Δ B (h2: [Δ |- t ≅ u : B]), #|h1| = #|h2|.
-  Let PTmRedEq (Γ : context) (A t u : term) (h1: [Γ |- t ≅h u : A]) :=
-    forall Δ B (h2: [Δ |- t ≅ u : B]), #|h1| = #|h2|.
-
-  Lemma algo_conv_size_unique : AlgoConvDepInductionConcl PTyEq PTyRedEq
-      PNeEq PNeRedEq PTmEq PTmRedEq.
-  Proof.
-    subst PTyEq PTyRedEq PNeEq PNeRedEq PTmEq PTmRedEq.
-    apply AlgoConvDepInduction.
-    - intros * ih ? h; destruct h as [?? A'' ? B'']; simpl_size.
-      pose proof c as []%algo_conv_wh.
-      pose proof c0 as []%algo_conv_wh.
-      assert (A' = A'') by (eapply whred_det ; tea; gen_typing).
-      assert (B' = B'') by (eapply whred_det ; tea; gen_typing).
-      subst. specialize (ih _ c0). lia.
-    - intros * ih1 * ih2 ? h2. depind h2; try discriminate.
-      2: pose proof c as []%algo_conv_wh; inv_whne.
-      refold. specialize (ih1 _ c); specialize (ih2 _ c0).
-      simpl_size; lia.
-    - intros ?? h; depind h; [reflexivity|].
-      refold. pose proof c as []%algo_conv_wh; inv_whne.
-    - intros ?? h; depind h; [reflexivity|].
-      refold. pose proof c as []%algo_conv_wh; inv_whne.
-    - intros ?? h; depind h; [reflexivity|].
-      refold. pose proof c as []%algo_conv_wh; inv_whne.
-    - intros * ih1 * ih2 ? h; depind h; refold.
-      2: pose proof c as []%algo_conv_wh; inv_whne.
-      specialize (ih1 _ c); specialize (ih2 _ c0).
-      simpl_size; lia.
-    - intros * ih ? h ; depind h; refold.
-      2: pose proof c as []%algo_conv_wh; inv_whne.
-      specialize (ih _ c); simpl_size; lia.
-    - intros * ih ? h. 
-      pose proof c as []%algo_conv_wh.
-      destruct h; try solve [inv_whne]; refold.
-      specialize (ih _ _ c0); simpl_size; lia.
-    - intros ?????? h; depind h.
-      2: cbn in i; inversion i.
-      epose (uip H eq_refl); subst.
-      cbn in *; subst; simpl_size; reflexivity.
-    - intros * ih1 * ih2 ?? h; depind h; refold.
-      2: cbn in i; inversion i.
-      specialize (ih1 _ _ c); specialize (ih2 _ _ c0); simpl_size; lia.
-    - intros * ih1 * ih2 * ih3 * ih4 ?? h; depind h; refold.
-      2: cbn in i; inversion i.
-      specialize (ih1 _ _ c); specialize (ih2 _ c0); 
-      specialize (ih3 _ _ c1); specialize (ih4 _ _ c2); 
-       simpl_size; lia.
-    - intros * ih1 * ih2 ?? h; depind h; refold. 
-      2: cbn in i; inversion i.
-      specialize (ih1 _ _ c); specialize (ih2 _ c0); simpl_size; lia.
-    - intros * ih ?? h; depind h; refold.
-      2: cbn in i; inversion i.
-      specialize (ih _ _ c);  simpl_size; lia.
-    - intros * ih ?? h; depind h; refold.
-      2: cbn in i; inversion i.
-      specialize (ih _ _ c);  simpl_size; lia.
-    - intros * ih1 * ih2 * ih3 ?? h; depind h; refold.
-      (* Uhh !!! *)
-      Fail match goal with [ H : (_ || _) |- _ ] => idtac H end.
-      all: try (cbn in i; solve [inversion i]).
-      1: cbn in i0; solve [inversion i0].
-      specialize (ih1 _ _ c). ; specialize (ih2 _ c0); 
-      specialize (ih3 _ _ c1);  simpl_size; lia.
-
-
-
-
-  
-End SizeUnicity.
-
-*)
